Hacl.Operations: support for in-place XOR function

crypto_hst/utils/Hacl.Operations.fst
@@ -1,14 +1,36 @@
 module Hacl.Operations
 
+open FStar.HyperStack
+open FStar.HST
+open FStar.Buffer
 open FStar.UInt32
 
 
 (* Define base types *)
 let u32 = FStar.UInt32.t
 let s32 = Hacl.UInt32.t
+let bytes = Hacl.SBuffer.u8s
 
 
 (* Define word functions *)
 let rotate_right (a:s32) (b:u32{v b <= 32}) : Tot s32 =
   Hacl.UInt32.logor (Hacl.UInt32.shift_right a b) (Hacl.UInt32.shift_left a (FStar.UInt32.sub 32ul b))
 
+
+(* Define helper xor function *)
+val xor_bytes: output:bytes -> in1:bytes{disjoint in1 output} -> 
+  len:u32{v len <= length output /\ v len <= length in1} -> STL unit
+  (requires (fun h -> live h output /\ live h in1))
+  (ensures  (fun h0 _ h1 -> live h0 output /\ live h0 in1 /\ live h1 output /\ live h1 in1
+    /\ modifies_1 output h0 h1 ))
+let rec xor_bytes output in1 len =
+  if len =^ 0ul then ()
+  else
+    begin
+      let i    = Hacl.UInt32.sub_mod len 1ul in
+      let in1i = index in1 i in
+      let oi   = index output i in
+      let oi   = Hacl.UInt8.logxor in1i oi in
+      upd output i oi;
+      xor_bytes output in1 i
+    end
